src/sf_lemmas.v
@@ -1,0 +1,593 @@
+Require sf_spec.
+Require Import sf_tactic.
+Require Import RelDec.
+Require Import List.
+Require Import Sorted.
+Require Import Permutation.
+Require Import FunctionalExtensionality.
+Require Import Classical.
+Import ListNotations.
+
+Section cand.
+
+Variable candidate : Set.
+Variable reldec_candidate : RelDec (@eq candidate).
+Variable reldec_correct_candidate : RelDec_Correct reldec_candidate.
+
+Ltac solve_rcv := sf_tactic.solve_rcv reldec_correct_candidate.
+Ltac intuition_nosplit := sf_tactic.intuition_nosplit reldec_correct_candidate.
+
+
+Lemma next_ranking_cons_or :
+forall b1 bal e x,
+sf_spec.next_ranking candidate e (b1 :: bal) x ->
+sf_spec.next_ranking candidate e [b1] x \/ 
+sf_spec.next_ranking candidate e bal x.
+intros. inv H; solve_rcv. left.
+destruct H4; solve_rcv. eapply sf_spec.next_ranking_valid; solve_rcv.
+left. eauto. eapply sf_spec.next_ranking_valid; solve_rcv.
+Qed.
+
+Lemma next_ranking_in :
+forall e bal x,
+  sf_spec.next_ranking candidate e bal x ->
+  In x bal.
+Proof.
+induction bal; solve_rcv.
+inv H; solve_rcv. 
+Qed.
+
+Lemma no_viable_candidates_cons :
+forall a b e,
+sf_spec.no_viable_candidates candidate (e) (a ::  b) <->
+(sf_spec.no_viable_candidates candidate e [a] /\
+sf_spec.no_viable_candidates candidate e b).
+split.
+intros.
+unfold sf_spec.no_viable_candidates in *.
+split.
+intros. eapply H; eauto. inv H0; simpl in *; intuition.
+intros. eapply H; eauto. simpl. intuition.
+intros. intuition.
+unfold sf_spec.no_viable_candidates in *. simpl in *.
+intuition. eapply H0; eauto. 
+eapply H1; eauto.
+Qed.
+
+Lemma first_choices_app : 
+forall c l1 l2 x1 x2  r cnd, 
+sf_spec.first_choices c r cnd l1 x1 ->
+sf_spec.first_choices c r cnd l2 x2 ->
+sf_spec.first_choices c r cnd (l1 ++ l2) (x1 + x2).
+Proof.
+induction l1; intros.
+- simpl in *. inv H. simpl. auto.
+- simpl in *. Print sf_spec.first_choices.
+  inv H.
+  + apply sf_spec.first_choices_selected. auto. fold plus.
+    apply IHl1; auto.
+  + apply sf_spec.first_choices_not_selected; auto.
+Qed.
+
+Lemma first_choices_app_gt :
+forall c l1 l2 x1 x2 r cnd,
+sf_spec.first_choices c r cnd l1 x1 ->
+sf_spec.first_choices c r cnd (l1 ++ l2) (x2) ->
+x2 >= x1.
+Proof.
+induction l1; intros.
+- simpl in *. inv H. omega.
+- simpl in *. inv H; inv H0; try congruence; try omega.
+  eapply IHl1 in H5; eauto. omega.
+  eapply IHl1; eauto.
+Qed.
+
+Lemma first_choices_perm : 
+forall c l1 l2 x r cnd,
+Permutation l1 l2 ->
+sf_spec.first_choices c r cnd l1 x ->
+sf_spec.first_choices c r cnd l2 x.
+Proof.
+induction l1; intros.
+- apply Permutation_nil in H. subst. auto. 
+- assert (exists l2s l23, l2 = l2s ++ (a :: l23)). 
+  { eapply Permutation_in in H. instantiate (1 := a) in H.
+    apply List.in_split in H. auto.
+    constructor; auto. }
+  destruct H1. destruct H1.
+  subst.
+  apply Permutation_cons_app_inv in H.
+  inv H0.
+  + eapply (IHl1 _ n' r cnd) in H; auto.
+    clear - H H3.
+    { generalize dependent x1. generalize dependent n'.
+      induction x0; intros.
+      - simpl in *. constructor; auto.
+      - simpl in *. inv H. 
+        + constructor; auto.
+        + apply sf_spec.first_choices_not_selected; auto.
+    }
+  + eapply IHl1 in H; eauto.
+    { clear - H H3.
+      generalize dependent x1. generalize dependent x.
+      induction x0; intros.
+      - simpl in *. apply sf_spec.first_choices_not_selected; auto.
+      - simpl in *. inv H.
+        + constructor; auto.
+        + apply sf_spec.first_choices_not_selected; auto.
+    }
+Qed.
+
+Lemma selected_participates : forall election (c : candidate) bal  r,
+sf_spec.selected_candidate _ r bal c ->
+In bal election ->
+sf_spec.participates _ c election.
+Proof.
+induction election; intros.
+inv H0.
+destruct H0. subst.
+unfold sf_spec.participates.
+unfold sf_spec.selected_candidate in H.
+destruct H. destruct H0.
+exists bal. split; eauto.
+simpl. auto.
+exists x. intuition.
+apply next_ranking_in in H1. auto.
+eapply IHelection in H0.
+unfold sf_spec.participates in H0.
+unfold sf_spec.participates.
+simpl in *.
+destruct H0.
+exists x. split; auto. intuition.
+destruct H0.
+apply H1.
+eauto.
+Qed.
+
+Lemma participates_cons : forall e a (c : candidate) ,
+        sf_spec.participates _ c [a] \/ sf_spec.participates _ c e <->
+        sf_spec.participates _ c (a :: e).
+Proof.
+split.
+- intros.
+  destruct H.
+  + unfold sf_spec.participates in *.
+    destruct H. destruct H. destruct H0. destruct H0.
+    exists a. simpl in *. intuition.
+    subst. exists x0. auto.
+  + unfold sf_spec.participates in *. 
+    destruct  H. intuition. destruct H1. exists x; intuition.
+    exists x0; intuition.
+- intros. destruct H.
+  destruct H. destruct H0.
+  destruct H.
+  +  unfold sf_spec.participates.
+     subst. left. exists x. intuition.
+     exists x0; auto.
+  +  right. unfold sf_spec.participates.
+     exists x. intuition.
+     exists x0; auto.
+Qed.
+
+Lemma total_selected_unique : forall r e v v',
+sf_spec.total_selected candidate r e v ->
+sf_spec.total_selected candidate r e v' ->
+v= v'.
+Admitted.
+
+Lemma majority_not_0 :
+forall r e x ,
+sf_spec.majority candidate r e x ->
+exists v, sf_spec.first_choices _ r x e v /\ v <> 0.
+Proof.
+intros.
+unfold sf_spec.majority in *.
+edestruct (sf_spec.sf_first_choices_total _ r e x).
+edestruct (sf_spec.total_selected_total _ r e).
+exists x0. intuition.
+subst.
+eapply H in H0; eauto.
+omega.
+Qed.
+
+Lemma update_eliminated_in_rec : forall rec loser c,
+sf_spec.update_eliminated candidate (in_record rec) loser c <->
+in_record ([loser] :: rec) c.
+Proof.
+split; intros.
+{ induction rec.
+  - unfold sf_spec.update_eliminated in H.
+    intuition. inv H0. destruct H. inv H.
+    subst. unfold in_record. exists [c]. intuition; auto.
+  - unfold sf_spec.update_eliminated in  *. intuition.
+    unfold in_record in H0. destruct H0. intuition.
+    simpl in H2. destruct H2.
+    + subst. unfold in_record. exists x. 
+      intuition.
+    + unfold in_record. exists x. intuition.
+    + unfold in_record in H2. destruct H2.
+      intuition. simpl in H2. destruct H2.
+      * subst. unfold in_record. exists [c].
+        intuition.
+      * exists x. intuition. }
+{ unfold in_record in H. destruct H. intuition. simpl in H0.
+  destruct H0. subst. unfold sf_spec.update_eliminated.
+  right. inv H1; auto. inv H.
+  left. unfold in_record. eauto. }
+Qed.
+
+Axiom prop_ext : forall (P Q : Prop), 
+  (P <-> Q) -> P = Q.
+
+
+Lemma update_eliminated_in_rec_eq : forall rec loser c,
+sf_spec.update_eliminated candidate (in_record rec) loser c =
+in_record ([loser] :: rec) c.
+Proof. intros.
+apply prop_ext. apply update_eliminated_in_rec.
+Qed.
+
+
+Lemma update_eliminated_in_rec_eq_noc : forall rec loser,
+sf_spec.update_eliminated candidate (in_record rec) loser =
+in_record ([loser] :: rec).
+intros. extensionality c. apply update_eliminated_in_rec_eq.
+Qed.
+
+Definition continuing2 b rec:=
+exists r, sf_spec.next_ranking candidate rec b r /\ ~sf_spec.overvote candidate r.
+
+
+Lemma continuing2_continuing : 
+forall b rec,
+continuing2 b rec <-> sf_spec.continuing_ballot candidate rec b.
+Proof.
+intros.
+split.
+intros.
+unfold continuing2 in *.
+solve_rcv.
+destruct H1. apply H1. exists x. auto.
+destruct H1. solve_rcv.
+eapply sf_spec.next_ranking_unique in H; eauto. subst.
+apply H0; eauto.
+intros.
+unfold continuing2.
+solve_rcv.
+
+apply Classical_Prop.not_or_and in H.
+destruct H. apply Classical_Prop.NNPP in H.
+destruct H. exists x.
+split. auto.
+intro. apply H0. exists x. auto.
+Qed.
+
+Lemma continuing_ballot_cons :
+forall r h t,
+sf_spec.continuing_ballot candidate r (h :: t) ->
+sf_spec.continuing_ballot candidate r [h] \/ ((~sf_spec.overvote candidate h) /\ sf_spec.continuing_ballot candidate r t).
+Proof.
+intros. repeat rewrite <- continuing2_continuing in *.
+induction t. 
+- auto.
+- unfold continuing2 in *.
+  destruct H. destruct H.
+  inv H.
+  + right. intuition. exists x. auto.
+  + destruct H5. 
+    *  intuition. 
+    * left. exists x.
+      intuition. eapply sf_spec.next_ranking_valid.
+      apply H3. auto.
+Qed.
+
+Lemma continuing_ballot_cons2 :
+forall r a b,
+sf_spec.continuing_ballot candidate r [a] ->
+sf_spec.continuing_ballot candidate r (a :: b).
+Proof.
+intros. rewrite <- continuing2_continuing in *.
+unfold continuing2 in *. destruct H.
+exists x.
+destruct H. intuition.
+clear H0.
+inv H. inv H5. eapply sf_spec.next_ranking_valid; eauto.
+Qed.
+
+Lemma continuing_ballot_cons3 :
+forall t h r
+(OV : ~sf_spec.overvote candidate h), 
+sf_spec.continuing_ballot candidate r t ->
+sf_spec.continuing_ballot candidate r (h :: t).
+Proof.
+intros. rewrite <- continuing2_continuing in *.
+unfold continuing2 in *.
+destruct H. destruct H.
+destruct (classic (Forall r h)).
+exists x. intuition. 
+constructor; eauto.
+destruct h. exfalso. solve_rcv. apply H1. solve_rcv.
+exists (c::h). intuition.
+eapply sf_spec.next_ranking_valid. simpl. eauto. 
+right. solve_rcv. apply H1. intros. destruct H3. subst. auto.
+destruct (rel_dec_p c x0).
+subst. auto.
+exfalso. apply OV. exists c. exists x0.
+simpl. auto.
+Qed.
+
+Lemma continuing_ballot_rec_cons : 
+forall l r b,
+  sf_spec.continuing_ballot candidate (in_record ([l] :: r)) (b) ->
+   sf_spec.continuing_ballot candidate (in_record r) (b).
+Proof.
+  intros. induction b.
+  - unfold sf_spec.continuing_ballot in *.  
+    intro. apply H. clear H.
+    unfold sf_spec.exhausted_ballot. left. intro.
+    inv H. inv H1.
+  - apply continuing_ballot_cons in H.  
+    destruct H.
+    apply continuing_ballot_cons2. 
+    rewrite <- continuing2_continuing in *.
+    unfold continuing2. 
+    unfold continuing2 in H.
+    destruct H. exists x.
+    destruct H. intuition.
+    inv H. constructor; solve_rcv.
+    destruct H5. intuition.
+    eapply sf_spec.next_ranking_valid; eauto.
+    right. intro. apply H; clear H.
+    unfold in_record in *. solve_rcv.
+    intuition.
+    apply continuing_ballot_cons3; auto.
+Qed.
+
+Lemma next_ranking_cons_or2 :
+forall b1 bal e x,
+sf_spec.next_ranking candidate e (b1 :: bal) x ->
+sf_spec.next_ranking candidate e [b1] x \/ 
+(Forall e b1 /\ sf_spec.next_ranking candidate e bal x).
+intros. inv H; solve_rcv. left.
+destruct H4; solve_rcv. eapply sf_spec.next_ranking_valid; solve_rcv.
+left. eauto. eapply sf_spec.next_ranking_valid; solve_rcv.
+Qed.
+
+Lemma continuing_ballot_cons4 : (*should be main lemma, don't want to rework proofs :( *)
+forall r h t,
+sf_spec.continuing_ballot candidate r (h :: t) ->
+sf_spec.continuing_ballot candidate r [h] \/ ((~sf_spec.overvote candidate h) /\ sf_spec.continuing_ballot candidate r t /\ Forall r h).
+Proof.
+intros. repeat rewrite <- continuing2_continuing in *.
+induction t. 
+- auto.
+- unfold continuing2 in *.
+  destruct H. destruct H.
+  inv H.
+  + right. intuition. exists x. auto.
+  + destruct H5. 
+    *  intuition. 
+    * left. exists x.
+      intuition. eapply sf_spec.next_ranking_valid.
+      apply H3. auto.
+Qed.
+
+Lemma selected_cons :
+forall r a b c,
+sf_spec.selected_candidate candidate  r (a :: b) c ->
+sf_spec.selected_candidate candidate r [a] c \/
+(Forall r a /\ ~sf_spec.overvote candidate a /\sf_spec.selected_candidate candidate r b c).
+Proof.
+intros.
+unfold sf_spec.selected_candidate in H.
+intuition_nosplit. apply continuing_ballot_cons4 in H.
+apply next_ranking_cons_or2 in H0.
+destruct H, H0.
+left. unfold sf_spec.selected_candidate. intuition.
+eauto.
+rewrite <- continuing2_continuing in H.
+unfold continuing2 in H. destruct H. destruct H.
+inv H. inv H8. rewrite Forall_forall in H0. intuition.
+destruct H. destruct H2. inv H0. inv H9. rewrite Forall_forall in *.
+intuition.
+right. unfold sf_spec.selected_candidate. intuition.
+eauto.
+Qed.
+
+Lemma first_choices_0_cons :
+forall r c h t,
+sf_spec.first_choices candidate r c (h :: t) 0 <->
+sf_spec.first_choices candidate r c [h] 0 /\
+sf_spec.first_choices candidate r c t 0.
+Proof.
+split.
+- intros.
+  induction t. intuition. constructor.
+  inv H. intuition.
+  inv H4.
+  apply IHt.
+  constructor. auto. auto.
+- intros. destruct H.
+  inv H. constructor; auto.
+Qed.
+
+Lemma next_ranking_record_same :
+forall b x c l r,
+  In c x ->
+  c <> l ->
+  sf_spec.next_ranking candidate (in_record r) b x ->
+  ~ sf_spec.overvote candidate x ->
+  sf_spec.next_ranking candidate (in_record ([l] :: r)) b x.
+Proof.
+induction b; intros.
+inv H1.
+inv H1.
+- constructor. solve_rcv. specialize (H5 x0); solve_rcv.
+  auto.
+  eapply IHb; eauto.
+- intuition.
+  eapply sf_spec.next_ranking_valid.
+  apply H5. right. intro.
+  apply H1. solve_rcv. simpl in H3. destruct H3; solve_rcv.
+  assert (c0 = l). inv H4. subst; intuition. inv H3. subst. clear H4.
+  exfalso. apply H2. exists c. exists l. eauto.
+Qed.
+
+Lemma ne_still_continuing :
+forall b c l  x r,
+sf_spec.next_ranking candidate (in_record r) b x ->
+sf_spec.continuing_ballot candidate (in_record r) b ->
+In c x ->
+c <> l ->
+sf_spec.continuing_ballot candidate (in_record ([l] :: r)) b.
+Proof.
+intros. repeat rewrite <- continuing2_continuing in *.
+unfold continuing2 in *. intuition_nosplit.
+exists x0. split; eauto. 
+eapply sf_spec.next_ranking_unique in H; eauto. subst.
+eapply next_ranking_record_same; eauto.
+Qed.
+
+Lemma selected_rec_cons :
+forall r b c l,
+c <> l ->
+sf_spec.selected_candidate candidate (in_record r) b c ->
+sf_spec.selected_candidate candidate (in_record ([l]::r)) b c.
+intros.
+induction b. solve_rcv.
+apply selected_cons in H0. 
+destruct H0. 
+- clear IHb. 
+  unfold sf_spec.selected_candidate in *.
+  intuition_nosplit.
+  split. 
+  + apply continuing_ballot_cons2. 
+  eapply ne_still_continuing; eauto.
+  + inv H1. inv H8.
+    destruct H7. exists x. intuition.
+    eapply sf_spec.next_ranking_valid; eauto.
+    exists x. intuition. eapply sf_spec.next_ranking_valid; eauto.
+    right. intro. apply H1. rewrite <- continuing2_continuing in *. 
+    unfold continuing2 in *. unfold in_record in *. intuition_nosplit. 
+    simpl in *. destruct H3; subst; try solve [solve_rcv].
+    inv H4; intuition_nosplit. inv H0. inv H10. intuition.
+    exfalso. apply H6. solve_rcv.
+- intuition. clear H3. 
+  unfold sf_spec.selected_candidate in *.
+  intuition_nosplit. split. 
+  rewrite <- continuing2_continuing. unfold continuing2. exists x.
+  intuition. constructor; auto. rewrite Forall_forall in *.
+  intro. specialize (H1 x0). intro. intuition. 
+  solve_rcv.  rewrite <-  continuing2_continuing in *.
+  unfold continuing2 in *. intuition_nosplit.
+  eapply sf_spec.next_ranking_unique in H2; eauto. subst.
+  auto.
+  exists x. intuition.
+  constructor; auto.
+  rewrite Forall_forall in *. intros. specialize (H1 x0). 
+  solve_rcv.
+Qed.
+
+Lemma first_choices_rec_0 :
+forall c l r e,
+  sf_spec.first_choices candidate (in_record ([l] :: r)) c e 0 ->
+  c <> l ->
+  sf_spec.first_choices candidate (in_record r) c e 0.
+Proof.
+intros.
+induction e.
+- constructor.
+- apply first_choices_0_cons in H. destruct H. intuition.
+  apply first_choices_0_cons. intuition.
+  inv H.
+  constructor. intro. apply H5. clear H5. 
+  apply selected_rec_cons; auto. constructor.
+Qed.
+
+
+
+Lemma first_choices_0_loser :
+forall c election l,
+~in_record l c ->
+sf_spec.participates _ c election ->
+sf_spec.first_choices candidate (in_record l) c election 0 ->
+sf_spec.is_loser _ (in_record l) election c.
+Proof.
+intros. unfold sf_spec.is_loser in *.
+split.
+- unfold sf_spec.viable_candidate. 
+  split.
+  + unfold in_record. intuition_nosplit. apply H. unfold in_record. eauto.
+  + auto.
+- intros. eapply sf_spec.sf_first_choices_unique in H1; eauto. subst. omega.
+Qed.
+
+Lemma in_record_nil_nil (c: candidate) :
+forall l, in_record l c <-> in_record ([] :: l) c.
+split; intros; unfold in_record in *;
+intuition_nosplit. exists x. simpl. intuition.
+inv H. inv H0. exists x; simpl; auto.
+Qed.
+
+Lemma in_record_nil_nil_eq :
+forall (l : list (list candidate)), in_record l = in_record ([] :: l).
+intros. extensionality c. apply prop_ext.
+apply in_record_nil_nil.
+Qed.
+
+Fixpoint flatten {A} (l : list (list A)) : list A :=
+match l with
+| h :: t => h ++ flatten t
+| nil => nil
+end.
+
+
+Lemma in_flatten :
+forall A (x: list A) l (c : A),
+(exists x, In x l /\ In c x) <-> In c (flatten l).
+split; intros.
+- induction l.
+  +  intuition_nosplit.
+  + intuition_nosplit. simpl in *. destruct H.
+    * subst. apply in_app_iff. auto.
+    * apply in_app_iff. right. apply IHl. eauto.
+- induction l.
+  inv H.
+  simpl in *. apply in_app_or in H. destruct H.
+  eauto.
+  edestruct IHl; eauto.
+  exists x0. intuition.
+Qed.
+
+Lemma in_record_flatten (c : candidate): 
+forall l, in_record l c <-> in_record ([flatten l]) c.
+Proof.
+split; intros;
+unfold in_record in *; intuition_nosplit.
+exists (flatten l). intuition. apply in_flatten; eauto.
+inv H. apply in_flatten in H0. auto. apply nil.
+inv H1.
+Qed.
+
+
+Lemma winner_eliminate_0s :
+forall election r winner l
+(NODUP : NoDup l),
+(forall c, in_record (r::l) c -> sf_spec.first_choices _ (in_record l) c election 0) ->
+sf_spec.winner candidate election (in_record (r ::l) ) winner ->
+sf_spec.winner candidate election (in_record l) winner.
+Proof.
+intros. 
+induction r; auto; intros. rewrite in_record_nil_nil_eq. auto.  
+destruct (classic (sf_spec.participates _ a election)).
+- destruct (classic (sf_spec.no_majority candidate (in_record l) election)).
+  + eapply sf_spec.winner_elimination.
+    auto. specialize (H a). eapply first_choices_0_loser in H. apply H.
+    
+    auto. unfold in_record. 
+Admitted. 
+(*exists (a::r). simpl; auto.
+    rewrite update_eliminated_in_rec_eq_noc. inv H0. admit. (* no majority conflicts with majority *)
+*)
+
+End cand.
